Test/dafny1/UltraFilter.dfy
@@ -1,0 +1,108 @@
+// ultra filter
+
+class UltraFilter<G> {
+  static function IsFilter(f: set<set<G>>, S: set<G>): bool
+  {
+    (forall A, B :: A in f && A <= B ==> B in f) &&
+    (forall C, D :: C in f && D in f ==> C * D in f) &&
+    S in f &&
+    {} !in f
+  }
+
+  static function IsUltraFilter(f: set<set<G>>, S: set<G>): bool
+  {
+    IsFilter(f, S) &&
+    (forall g :: IsFilter(g, S) && f <= g ==> f == g)
+  }
+
+  method Theorem(f: set<set<G>>, S: set<G>, M: set<G>, N: set<G>)
+    requires IsUltraFilter(f, S);
+    requires M + N in f;
+    ensures M in f || N in f;
+  {
+    if (M !in f) {
+      // instantiate 'g' with the following 'h'
+      call h := H(f, S, M);
+      call Lemma_HIsFilter(h, f, S, M);
+      call Lemma_FHOrdering0(h, f, S, M);
+    }
+  }
+
+  // Dafny currently does not have a set comprehension expression, so this method stub will have to do
+  method H(f: set<set<G>>, S: set<G>, M: set<G>) returns (h: set<set<G>>);
+    ensures (forall X :: X in h <==> M + X in f);
+
+  method Lemma_HIsFilter(h: set<set<G>>, f: set<set<G>>, S: set<G>, M: set<G>)
+    requires IsFilter(f, S);
+    requires (forall X :: X in h <==> M + X in f);
+    requires M !in f;
+    ensures IsFilter(h, S);
+  {
+    // call Lemma_H0(h, f, S, M, *, *);
+    assume (forall A, B :: A in h && A <= B ==> B in h);
+
+    // call Lemma_H1(h, f, S, M, *, *);
+    assume (forall C, D :: C in h && D in h ==> C * D in h);
+
+    call Lemma_H2(h, f, S, M);
+
+    call Lemma_H3(h, f, S, M);
+  }
+
+  method Lemma_H0(h: set<set<G>>, f: set<set<G>>, S: set<G>, M: set<G>, A: set<G>, B: set<G>)
+    requires IsFilter(f, S);
+    requires (forall X :: X in h <==> M + X in f);
+    requires A in h && A <= B;
+    ensures B in h;
+  {
+    assert M + A <= M + B;
+  }
+
+  method Lemma_H1(h: set<set<G>>, f: set<set<G>>, S: set<G>, M: set<G>, C: set<G>, D: set<G>)
+    requires IsFilter(f, S);
+    requires (forall X :: X in h <==> M + X in f);
+    requires C in h && D in h;
+    ensures C * D in h;
+  {
+    assert (M + C) * (M + D) == M + (C * D);
+  }
+
+  method Lemma_H2(h: set<set<G>>, f: set<set<G>>, S: set<G>, M: set<G>)
+    requires IsFilter(f, S);
+    requires (forall X :: X in h <==> M + X in f);
+    ensures S in h;
+  {
+    // S is intended to stand for the universal set, but this is the only place where that plays a role
+    assume M <= S;
+
+    assert M + S == S;
+  }
+
+  method Lemma_H3(h: set<set<G>>, f: set<set<G>>, S: set<G>, M: set<G>)
+    requires IsFilter(f, S);
+    requires (forall X :: X in h <==> M + X in f);
+    requires M !in f;
+    ensures {} !in h;
+  {
+    assert M + {} == M;
+  }
+
+  method Lemma_FHOrdering0(h: set<set<G>>, f: set<set<G>>, S: set<G>, M: set<G>)
+    requires IsFilter(f, S);
+    requires (forall X :: X in h <==> M + X in f);
+    requires IsFilter(h, S);
+    ensures f <= h;
+  {
+    // call Lemma_FHOrdering1(h, f, S, M, *);
+    assume (forall Y :: Y in f ==> Y in h);
+    assume f <= h;  // hickup in boxing
+  }
+
+  method Lemma_FHOrdering1(h: set<set<G>>, f: set<set<G>>, S: set<G>, M: set<G>, Y: set<G>)
+    requires IsFilter(f, S);
+    requires (forall X :: X in h <==> M + X in f);
+    ensures Y in f ==> Y in h;
+  {
+    assert Y <= M + Y;
+  }
+}
