Test/dafny0/runtest.bat
@@ -11,19 +11,10 @@ for %%f in (Simple.dfy) do (
   %DAFNY_EXE% %* /dprint:- /env:0 /noVerify %%f
 )
 
-for %%f in (BQueue.bpl) do (
-  echo.
-  echo -------------------- %%f --------------------
-  %BPLEXE% %* %%f
-)
-
 for %%f in (TypeTests.dfy SmallTests.dfy Definedness.dfy Array.dfy
-            Modules0.dfy Modules1.dfy BadFunction.dfy Queue.dfy ListCopy.dfy
-            BinaryTree.dfy ListReverse.dfy ListContents.dfy
-            SchorrWaite.dfy Termination.dfy Use.dfy DTypes.dfy
-            TypeParameters.dfy Datatypes.dfy UnboundedStack.dfy
-            SumOfCubes.dfy TerminationDemos.dfy Substitution.dfy
-            Tree.dfy Celebrity.dfy) do (
+            Modules0.dfy Modules1.dfy BadFunction.dfy
+            Termination.dfy Use.dfy DTypes.dfy
+            TypeParameters.dfy Datatypes.dfy) do (
   echo.
   echo -------------------- %%f --------------------
   %DAFNY_EXE% /compile:0 %* %%f
