Test/dafny1/runtest.bat
@@ -1,0 +1,26 @@
+@echo off
+setlocal
+
+set BOOGIEDIR=..\..\Binaries
+set DAFNY_EXE=%BOOGIEDIR%\Dafny.exe
+set BPLEXE=%BOOGIEDIR%\Boogie.exe
+
+for %%f in (BQueue.bpl) do (
+  echo.
+  echo -------------------- %%f --------------------
+  %BPLEXE% %* %%f
+)
+
+for %%f in (Queue.dfy
+            BinaryTree.dfy
+            UnboundedStack.dfy
+            ListCopy.dfy ListReverse.dfy ListContents.dfy
+            SchorrWaite.dfy
+            SumOfCubes.dfy
+            TerminationDemos.dfy Substitution.dfy TreeDatatype.dfy
+            Celebrity.dfy
+            UltraFilter.dfy) do (
+  echo.
+  echo -------------------- %%f --------------------
+  %DAFNY_EXE% /compile:0 %* %%f
+)
